src/hls/Gible.v
@@ -43,6 +43,8 @@ Require Import Predicate.
 Require Import Vericertlib.
 
 Definition node := positive.
+Definition predicate := positive.
+Definition pred_op := @pred_op predicate.
 
 (*|
 .. index::
